<?xml version="1.0"?>


<!DOCTYPE rdf:RDF [
    <!ENTITY owl "http://www.w3.org/2002/07/owl#" >
    <!ENTITY mlt "http://www.nemo.inf.ufes.br/mlt#" >
    <!ENTITY xsd "http://www.w3.org/2001/XMLSchema#" >
    <!ENTITY rdfs "http://www.w3.org/2000/01/rdf-schema#" >
    <!ENTITY rdf "http://www.w3.org/1999/02/22-rdf-syntax-ns#" >
]>


<rdf:RDF xmlns="http://www.nemo.inf.ufes.br/mlt#"
     xml:base="http://www.nemo.inf.ufes.br/mlt"
     xmlns:rdfs="http://www.w3.org/2000/01/rdf-schema#"
     xmlns:mlt="http://www.nemo.inf.ufes.br/mlt#"
     xmlns:owl="http://www.w3.org/2002/07/owl#"
     xmlns:xsd="http://www.w3.org/2001/XMLSchema#"
     xmlns:rdf="http://www.w3.org/1999/02/22-rdf-syntax-ns#">
    <owl:Ontology rdf:about="http://www.nemo.inf.ufes.br/mlt#">
        <owl:imports rdf:resource="http://www.w3.org/2000/01/rdf-schema#"/>
    </owl:Ontology>
    


    <!-- 
    ///////////////////////////////////////////////////////////////////////////////////////
    //
    // Object Properties
    //
    ///////////////////////////////////////////////////////////////////////////////////////
     -->

    


    <!-- http://www.nemo.inf.ufes.br/mlt#characterizes -->

    <owl:ObjectProperty rdf:about="&mlt;characterizes">
        <rdfs:comment>The principle of application of t1 defines that its instances applies to instances of t2 according a specific classification criteria. Thus, the extension of t1 is composed by the proper specializations of t2 that follows the specified classification criteria.</rdfs:comment>
        <rdfs:isDefinedBy rdf:resource="http://www.nemo.inf.ufes.br/mlt#"/>
        <rdfs:subPropertyOf rdf:resource="&mlt;crossLevelProperty"/>
        <rdfs:range>
            <owl:Class>
                <owl:unionOf rdf:parseType="Collection">
                    <rdf:Description rdf:about="&mlt;1stOrderClass"/>
                    <rdf:Description rdf:about="&mlt;2ndOrderClass"/>
                    <rdf:Description rdf:about="&mlt;TokenIndividual"/>
                </owl:unionOf>
            </owl:Class>
        </rdfs:range>
        <rdfs:domain>
            <owl:Class>
                <owl:unionOf rdf:parseType="Collection">
                    <rdf:Description rdf:about="&mlt;1stOrderClass"/>
                    <rdf:Description rdf:about="&mlt;2ndOrderClass"/>
                    <rdf:Description rdf:about="&mlt;3rdOrderClass"/>
                </owl:unionOf>
            </owl:Class>
        </rdfs:domain>
    </owl:ObjectProperty>
    


    <!-- http://www.nemo.inf.ufes.br/mlt#completelyCharacterizes -->

    <owl:ObjectProperty rdf:about="&mlt;completelyCharacterizes">
        <rdfs:comment>A variation of characterization in which the classification criteria defined by the principle of application of t1 guarantees that each instance of t2 is instance of at least one instance of t1.</rdfs:comment>
        <rdfs:isDefinedBy rdf:resource="http://www.nemo.inf.ufes.br/mlt#"/>
        <rdfs:subPropertyOf rdf:resource="&mlt;characterizes"/>
        <owl:propertyDisjointWith rdf:resource="&mlt;incompletelyCharacterizes"/>
    </owl:ObjectProperty>
    


    <!-- http://www.nemo.inf.ufes.br/mlt#crossLevelProperty -->

    <owl:ObjectProperty rdf:about="&mlt;crossLevelProperty">
        <rdfs:isDefinedBy rdf:resource="http://www.nemo.inf.ufes.br/mlt#"/>
        <rdfs:subPropertyOf rdf:resource="&mlt;multiLevelProperty"/>
    </owl:ObjectProperty>
    


    <!-- http://www.nemo.inf.ufes.br/mlt#disjointlyCharacterizes -->

    <owl:ObjectProperty rdf:about="&mlt;disjointlyCharacterizes">
        <rdfs:comment>A variation of characterization in which the classification criteria defined by the principle of application of t1 guarantees that each instance of t2 is instance of at most one instance of t1.</rdfs:comment>
        <rdfs:isDefinedBy rdf:resource="http://www.nemo.inf.ufes.br/mlt#"/>
        <rdfs:subPropertyOf rdf:resource="&mlt;characterizes"/>
        <owl:propertyDisjointWith rdf:resource="&mlt;overlappinglyCharacterizes"/>
    </owl:ObjectProperty>
    


    <!-- http://www.nemo.inf.ufes.br/mlt#incompletelyCharacterizes -->

    <owl:ObjectProperty rdf:about="&mlt;incompletelyCharacterizes">
        <rdfs:isDefinedBy rdf:resource="http://www.nemo.inf.ufes.br/mlt#"/>
        <rdfs:subPropertyOf rdf:resource="&mlt;characterizes"/>
    </owl:ObjectProperty>
    


    <!-- http://www.nemo.inf.ufes.br/mlt#intraLevelProperty -->

    <owl:ObjectProperty rdf:about="&mlt;intraLevelProperty">
        <rdfs:isDefinedBy rdf:resource="http://www.nemo.inf.ufes.br/mlt#"/>
        <rdfs:subPropertyOf rdf:resource="&mlt;multiLevelProperty"/>
    </owl:ObjectProperty>
    


    <!-- http://www.nemo.inf.ufes.br/mlt#isPowertypeOf -->

    <owl:ObjectProperty rdf:about="&mlt;isPowertypeOf">
        <rdfs:comment>The principle of application of t1 defines that its instances applies to instances of t2 but does not define a classification criteria. Thus, the extension of t1 is composed by all specializations of t2, including t2 itself.</rdfs:comment>
        <rdfs:isDefinedBy rdf:resource="http://www.nemo.inf.ufes.br/mlt#"/>
        <rdfs:subPropertyOf rdf:resource="&mlt;crossLevelProperty"/>
        <rdfs:domain>
            <owl:Class>
                <owl:unionOf rdf:parseType="Collection">
                    <rdf:Description rdf:about="&mlt;1stOrderClass"/>
                    <rdf:Description rdf:about="&mlt;2ndOrderClass"/>
                    <rdf:Description rdf:about="&mlt;3rdOrderClass"/>
                </owl:unionOf>
            </owl:Class>
        </rdfs:domain>
        <rdfs:range>
            <owl:Class>
                <owl:unionOf rdf:parseType="Collection">
                    <rdf:Description rdf:about="&mlt;1stOrderClass"/>
                    <rdf:Description rdf:about="&mlt;2ndOrderClass"/>
                    <rdf:Description rdf:about="&mlt;TokenIndividual"/>
                </owl:unionOf>
            </owl:Class>
        </rdfs:range>
    </owl:ObjectProperty>
    


    <!-- http://www.nemo.inf.ufes.br/mlt#isSubordinatedTo -->

    <owl:ObjectProperty rdf:about="&mlt;isSubordinatedTo">
        <rdfs:comment>The principle of application of each instance of t1 adds some classification criteria to the principle of application of some instance of t2 i.e. every instance of t1 proper specializes some instance of t2.
Domain and Range: Higher-order types of the same order (instances of 2ndOT or 3rdOT).</rdfs:comment>
        <rdfs:isDefinedBy rdf:resource="http://www.nemo.inf.ufes.br/mlt#"/>
        <rdfs:subPropertyOf rdf:resource="&mlt;intraLevelProperty"/>
        <rdfs:range>
            <owl:Class>
                <owl:unionOf rdf:parseType="Collection">
                    <rdf:Description rdf:about="&mlt;2ndOrderClass"/>
                    <rdf:Description rdf:about="&mlt;3rdOrderClass"/>
                </owl:unionOf>
            </owl:Class>
        </rdfs:range>
        <rdfs:domain>
            <owl:Class>
                <owl:unionOf rdf:parseType="Collection">
                    <rdf:Description rdf:about="&mlt;2ndOrderClass"/>
                    <rdf:Description rdf:about="&mlt;3rdOrderClass"/>
                </owl:unionOf>
            </owl:Class>
        </rdfs:domain>
    </owl:ObjectProperty>
    


    <!-- http://www.nemo.inf.ufes.br/mlt#multiLevelProperty -->

    <owl:ObjectProperty rdf:about="&mlt;multiLevelProperty">
        <rdfs:isDefinedBy rdf:resource="http://www.nemo.inf.ufes.br/mlt#"/>
    </owl:ObjectProperty>
    


    <!-- http://www.nemo.inf.ufes.br/mlt#overlappinglyCharacterizes -->

    <owl:ObjectProperty rdf:about="&mlt;overlappinglyCharacterizes">
        <rdfs:isDefinedBy rdf:resource="http://www.nemo.inf.ufes.br/mlt#"/>
        <rdfs:subPropertyOf rdf:resource="&mlt;characterizes"/>
    </owl:ObjectProperty>
    


    <!-- http://www.nemo.inf.ufes.br/mlt#partitions -->

    <owl:ObjectProperty rdf:about="&mlt;partitions">
        <rdfs:comment>Equivalent to the MLT Cross-level structural relation: completelyCharacterizes and disjointlyCharacterizes. A variation of characterization in which the classification criteria defined by the principle of application of t1 guarantees that each instance of t2 is instance of exactly one instance of t1.</rdfs:comment>
        <rdfs:isDefinedBy rdf:resource="http://www.nemo.inf.ufes.br/mlt#"/>
        <rdfs:subPropertyOf rdf:resource="&mlt;characterizes"/>
    </owl:ObjectProperty>
    


    <!-- http://www.nemo.inf.ufes.br/mlt#properSpecializes -->

    <owl:ObjectProperty rdf:about="&mlt;properSpecializes">
        <rdfs:subPropertyOf rdf:resource="&rdfs;subClassOf"/>
    </owl:ObjectProperty>
    


    <!-- 
    ///////////////////////////////////////////////////////////////////////////////////////
    //
    // Classes
    //
    ///////////////////////////////////////////////////////////////////////////////////////
     -->

    


    <!-- http://www.nemo.inf.ufes.br/mlt#1stOrderClass -->

    <owl:Class rdf:about="&mlt;1stOrderClass">
        <rdfs:label>1stOrderClass</rdfs:label>
        <rdfs:subClassOf rdf:resource="&rdfs;Class"/>
        <rdfs:comment>Particular entities, which are not types, are considered individuals. An entity is an instance of “Individual” iff it is not possibly related to another entity through instantiation.</rdfs:comment>
        <rdfs:isDefinedBy rdf:resource="http://www.nemo.inf.ufes.br/mlt#"/>
    </owl:Class>
    


    <!-- http://www.nemo.inf.ufes.br/mlt#2ndOrderClass -->

    <owl:Class rdf:about="&mlt;2ndOrderClass">
        <rdfs:label>2ndOrderClass</rdfs:label>
        <rdfs:subClassOf rdf:resource="&rdfs;Class"/>
        <rdfs:comment>An entity t is a second-order type iff all its instances are first-order types.</rdfs:comment>
        <rdfs:isDefinedBy rdf:resource="http://www.nemo.inf.ufes.br/mlt#"/>
    </owl:Class>
    


    <!-- http://www.nemo.inf.ufes.br/mlt#3rdOrderClass -->

    <owl:Class rdf:about="&mlt;3rdOrderClass">
        <rdfs:label>3rdOrderClass</rdfs:label>
        <rdfs:subClassOf rdf:resource="&rdfs;Class"/>
        <rdfs:comment>An entity t is a third-order type iff all its instances are second-order types.</rdfs:comment>
        <rdfs:isDefinedBy rdf:resource="http://www.nemo.inf.ufes.br/mlt#"/>
    </owl:Class>
    


    <!-- http://www.nemo.inf.ufes.br/mlt#TokenIndividual -->

    <owl:Class rdf:about="&mlt;TokenIndividual">
        <rdfs:label>TokenIndividual</rdfs:label>
        <rdfs:comment>An entity whose instances are instances of Token Individual.</rdfs:comment>
    </owl:Class>
    


    <!-- http://www.w3.org/2000/01/rdf-schema#Class -->

    <owl:Class rdf:about="&rdfs;Class"/>
    


    <!-- 
    ///////////////////////////////////////////////////////////////////////////////////////
    //
    // Individuals
    //
    ///////////////////////////////////////////////////////////////////////////////////////
     -->

    


    <!-- http://www.nemo.inf.ufes.br/mlt#1stOrderClass -->

    <owl:NamedIndividual rdf:about="&mlt;1stOrderClass">
        <rdf:type rdf:resource="&mlt;2ndOrderClass"/>
    </owl:NamedIndividual>
    


    <!-- http://www.nemo.inf.ufes.br/mlt#2ndOrderClass -->

    <owl:NamedIndividual rdf:about="&mlt;2ndOrderClass">
        <rdf:type rdf:resource="&mlt;3rdOrderClass"/>
    </owl:NamedIndividual>
    


    <!-- http://www.nemo.inf.ufes.br/mlt#TokenIndividual -->

    <owl:NamedIndividual rdf:about="&mlt;TokenIndividual">
        <rdf:type rdf:resource="&mlt;1stOrderClass"/>
    </owl:NamedIndividual>
    


    <!-- 
    ///////////////////////////////////////////////////////////////////////////////////////
    //
    // General axioms
    //
    ///////////////////////////////////////////////////////////////////////////////////////
     -->

    <rdf:Description>
        <rdf:type rdf:resource="&owl;AllDisjointClasses"/>
        <owl:members rdf:parseType="Collection">
            <rdf:Description rdf:about="&mlt;1stOrderClass"/>
            <rdf:Description rdf:about="&mlt;2ndOrderClass"/>
            <rdf:Description rdf:about="&mlt;3rdOrderClass"/>
            <rdf:Description rdf:about="&mlt;TokenIndividual"/>
        </owl:members>
    </rdf:Description>
</rdf:RDF>



<!-- Generated by the OWL API (version 3.4.2) http://owlapi.sourceforge.net -->

